End of day 14/06/18

michael_formal/EFSM_LTL.thy
@@ -9,21 +9,11 @@ definition step :: "efsm \<Rightarrow> statename \<Rightarrow> registers \<Right
     _ \<Rightarrow> (0, [], r)"
 
 abbreviation neXt :: "efsm \<Rightarrow> statename \<Rightarrow> registers \<Rightarrow> event \<Rightarrow> ((statename \<times> outputs \<times> registers) \<Rightarrow> event \<Rightarrow> bool) \<Rightarrow> bool" where
-  "neXt e s r h f \<equiv> f (step e s r (fst h) (snd h)) h"
+  "neXt e s r v f \<equiv> f (step e s r (fst v) (snd v)) v"
 
 primrec globally :: "efsm \<Rightarrow> (statename \<times> outputs \<times> registers) \<Rightarrow> trace \<Rightarrow> (statename \<Rightarrow> event \<Rightarrow> registers \<Rightarrow> outputs \<Rightarrow> bool) \<Rightarrow> bool" where
   "globally e spr [] f = f (fst spr) ('''', []) (snd (snd spr)) (fst (snd spr))" |
   "globally e spr (h#t) f = conj (f (fst spr) h (snd (snd spr)) (fst (snd spr))) (globally e (step e (fst spr) (snd (snd spr)) (fst h) (snd h)) t f)"
-
-(*
-noChangeOwner: THEOREM filesystem |- FORALL (user : UID): G(cfstate /= NULL_STATE) => 
-G( 
-  (label=write AND r_1=user AND ip_1_write_1/=accessDenied) => 
-  G((cfstate=S_2 AND label=read AND r_1/=user) => 
-    X(op_1_read_0 = accessDenied) 
-  ) 
-  );
-*)
 
 lemma read_not_none : "\<forall>r'. step filesystem 2 r ''read'' [] \<noteq> (0, [], r')"
   by (simp add: fs_simp step_def)
@@ -69,8 +59,7 @@ lemma read_denied1: "r ''r1'' \<noteq> r ''r3'' \<Longrightarrow> EFSM_LTL.step 
   apply (simp add: fs_simp step_def)
   by (rule ext, simp)
 
-lemma read_step: "EFSM_LTL.step filesystem 2 r ''read'' [] = (2, [r ''r2''], r) \<or>
-EFSM_LTL.step filesystem 2 r ''read'' [] = (2, [0], r)"
+lemma read_step: "step filesystem 2 r ''read'' [] = (2, [r ''r2''], r) \<or> step filesystem 2 r ''read'' [] = (2, [0], r)"
   apply (case_tac "r ''r1'' = r ''r3''")
    apply (simp add: read_success)
   by (simp add: read_denied1)
@@ -108,6 +97,70 @@ case Nil
 next
   case (Cons a t)
   then show ?case by simp
+qed
+
+lemma login_1: "fst a = ''login'' \<and> length (snd a) = Suc 0 \<Longrightarrow> step filesystem 1 r ''login'' (snd a) = (2, [], (\<lambda>x. if x = ''r1'' then hd (snd a) else r x))"
+  apply (simp add: fs_simp step_def)
+  apply (rule ext)
+  by (simp add: index2state_i1)
+
+lemma login_user_1: "EFSM_LTL.step filesystem 1 reg ''login'' [1] = (2, [], (\<lambda>x. if x = ''r1'' then 1 else reg x))"
+  apply (simp add: fs_simp step_def)
+  apply (rule ext)
+  by simp
+
+(*
+noChangeOwner: THEOREM filesystem |- FORALL (user : UID): 
+G(cfstate /= NULL_STATE) => 
+G( 
+  (label=write AND r_1=user AND ip_1_write_1/=accessDenied) => 
+  G((cfstate=S_2 AND label=read AND r_1/=user) => 
+    X(op_1_read_0 = accessDenied) 
+  ) 
+  );
+*)
+
+lemma "globally filesystem (state, outs, r) t (\<lambda>s e r p. s \<noteq> 0) \<longrightarrow>
+globally filesystem (state, outs, reg) t (\<lambda>s e r p. (fst e = ''write'' \<and> r ''r1'' = 1 \<and> snd e \<noteq> [0]) \<longrightarrow>
+  globally filesystem (state, outs, reg) t (\<lambda>s' e' r' p'. (s' = 2 \<and> fst e' = ''read'' \<and> r' ''r1'' \<noteq> 1)\<longrightarrow>
+    (fst (snd (step filesystem s' r' (fst e') (snd e')))) = [0])
+)"
+proof (induction t)
+  case Nil
+  then show ?case by simp
+next
+  case (Cons a t')
+  then show ?case
+    apply simp
+    apply (case_tac "state = 0") (* If we're in state zero, it doesn't matter *)
+     apply (simp)
+    apply (case_tac "state = 1") (* If we were in state 1 to start with and prepend something *)
+     apply simp
+     apply (case_tac "fst a = ''login'' \<and> length (snd a) = 1")
+    apply simp
+
+qed
+
+lemma "\<forall> outs. globally filesystem (state, outs, r) t (\<lambda>s e r p. s \<noteq> 0) \<longrightarrow>
+globally filesystem (state, outs, r) t (\<lambda>s e r p. (fst e = ''write'' \<and> r' ''r1'' = 1 \<and> snd e \<noteq> [0]) \<longrightarrow>
+  globally filesystem (state, outs, r) t (\<lambda>s e r p. (s = 2 \<and> fst e = ''read'' \<and> r' ''r1'' \<noteq> 1)) \<longrightarrow>
+    neXt filesystem state r (hd t) (\<lambda>spr e. (fst (snd spr)) = [0])
+)"
+proof (induction t)
+  case Nil
+  then show ?case by simp
+next
+  case (Cons a t')
+  then show ?case
+    apply simp
+    apply (case_tac "state = 0", simp)
+    apply (case_tac "state = 1", simp)
+     apply (case_tac "fst a = ''login'' \<and> length (snd a) = 1")
+      apply (simp add: truefun)
+     apply (simp add: truefun)
+    apply (case_tac "state = 2", simp)
+     apply (simp add: truefun)
+    by (simp add: truefun)
 qed
 
 lemma "all (t) (\<lambda>e. e = (''read'', []) \<or> e = (''login'', []) \<or> e = (''logout'', []) \<or> (fst e = ''write'' \<and> length (snd e) = 1)) \<Longrightarrow>
