michael_formal/EFSM_LTL_Inf.thy
@@ -1,0 +1,11 @@
+theory EFSM_LTL_Inf
+imports EFSM
+begin
+
+codatatype (sset:'a) stream = SCons (shd:'a) (stl: "'a stream") for
+  map: smap
+  rel: stream_all2
+
+primcorec siterate :: "('a \<Rightarrow> 'a) \<Rightarrow> 'a \<Rightarrow> 'a stream" where
+  "siterate g x = SCons x (siterate g (g x))"
+end
